timing/examples/FreeRTOS/tasks/eTaskGetState.v
@@ -1,80 +1,80 @@
-Require Import RTOSDemo_NoAsserts_Clz.
-Require Import riscvTiming.
+Require Import RTOSDemo.
+Require Import RISCVTiming.
 Import RISCVNotations.
-Require Import timing_auto.
 
-Module eTaskGetStateTime <: TimingModule.
-    Definition time_of_addr (s : store) (a : addr) : N :=
-        match neorv32_cycles_upper_bound s (RTOSDemo_NoAsserts_Clz a) with
-        | Some x => x | _ => 999 end.
+Module TimingProof (cpu : CPUTimingBehavior).
 
+Module Program_eTaskGetState <: ProgramInformation.
     Definition entry_addr : N := 0x80000958.
 
     Definition exits (t:trace) : bool :=
-    match t with (Addr a,_)::_ => match a with
-    | 0x800009e8 | 0x800009f0 => true
-    | _ => false
-  end | _ => false end.
-End eTaskGetStateTime.
+        match t with (Addr a,_)::_ => match a with
+        | 0x800009e8 | 0x800009f0 => true
+        | _ => false
+    end | _ => false end.
 
-Module eTaskGetStateAuto := TimingAutomation eTaskGetStateTime.
-Import eTaskGetStateTime eTaskGetStateAuto.
+    Definition binary := RTOSDemo.
+End Program_eTaskGetState.
 
-Definition pxCurrentTCB (gp : N) (mem : addr -> N) : N :=
+Module RISCVTiming := RISCVTiming cpu Program_eTaskGetState.
+Module eTaskGetStateAuto := RISCVTimingAutomation RISCVTiming.
+Import Program_eTaskGetState eTaskGetStateAuto.
+
+Definition pxCurrentTCB (gp : N) (mem : memory) : N :=
     mem Ⓓ[gp ⊖ 1896].
 
-Definition time_of_eTaskGetState (mem : addr -> N) (gp a3 : N) (xTask : addr) (t : trace) :=
+Definition time_of_eTaskGetState (mem : memory) (gp a3 : N) (xTask : addr) (t : trace) :=
   cycle_count_of_trace t =
-    time_mem + 2 +
+    tlw + taddi +
     if (pxCurrentTCB gp mem =? xTask) then (
-      time_branch + 2 + time_branch
+      ttbeq + taddi + tjalr
     ) else (
-      3 + 3 + 2 * time_mem + 2 + 3 * time_mem +
+      tfbeq + tcsrrci + tlw + tlw + tlui + tlw + tlw + tlw +
       if (mem Ⓓ[0x80080004] =? 0) then (
-        3 + 3
+        ttbne + tcsrrsi
       ) else (
-        time_branch
+        ttbne
       ) +
-      2 + 2 +
+      taddi + taddi +
       if (xTask ⊕ 40 =? gp ⊖ 984) then (
-        time_branch + time_branch
+        ttbeq + tjalr
       ) else (
-        3 + 2 +
+        tfbeq + taddi +
         if (xTask ⊕ 20 =? mem Ⓓ[gp ⊖ 1900]) then (
-          time_branch + time_branch
+          ttbeq + tjalr
         ) else (
-          3 + if (xTask ⊕ 20 =? mem Ⓓ[gp ⊖ 1904]) then (
-            time_branch + time_branch
+          tfbeq + if (xTask ⊕ 20 =? mem Ⓓ[gp ⊖ 1904]) then (
+            ttbeq + tjalr
           ) else (
-            3 + 2 + if (xTask ⊕ 20 =? gp ⊖ 1024) then (
-              3 + time_mem + 
+            tfbeq + taddi + if (xTask ⊕ 20 =? gp ⊖ 1024) then (
+              tfbne + tlw +
               if (xTask ⊕ 20 =? 0) then (
-                3 + time_mem + 2 +
+                tfbne + tlbu + taddi +
                 if (99 =? xTask ⊕ 20) then (
-                    time_branch + time_branch
+                    ttbeq + tjalr
                 ) else (
-                    3 + time_mem + if (99 =? xTask ⊕ 20) then (
-                        time_branch + time_branch
+                    tfbeq + tlbu + if (99 =? xTask ⊕ 20) then (
+                        ttbeq + tjalr
                     ) else (
-                        3 + time_mem + if (99 =? xTask ⊕ 20) then (
-                            time_branch + time_branch
+                        tfbeq + tlbu + if (99 =? xTask ⊕ 20) then (
+                            ttbeq + tjalr
                         ) else (
-                            3 + 2 + time_branch
+                            tfbeq + taddi + tjalr
                         )
                     )
                 )
               ) else (
-                time_branch + time_branch
+                ttbeq + tjalr
               )
             ) else (
-              time_branch + 2 + 2 +
+              ttbne + taddi + taddi +
               if (xTask ⊕ 20 =? gp ⊖ 1004) then (
-                time_branch + time_branch
+                ttbeq + tjalr
               ) else (
                 if (xTask ⊕ 20 =? 0) then (
-                  time_branch + time_branch
+                  ttbeq + tjalr
                 ) else (
-                  3 + 2 + time_branch
+                  tfbeq + taddi + tjalr
                 )
               )
             )
@@ -83,40 +83,33 @@ Definition time_of_eTaskGetState (mem : addr -> N) (gp a3 : N) (xTask : addr) (t
       )
     ).
 
-Definition eTaskGetState_timing_invs (s : store) (base_mem : addr -> N) (gp : N)
+Definition eTaskGetState_timing_invs (s : store) (base_mem : memory) (gp : N)
     (a3 : N) (xTask : addr) (t:trace) : option Prop :=
 match t with (Addr a, s) :: t' => match a with
-| 0x80000958 => Some (s V_MEM32 = Ⓜbase_mem /\ s R_GP = Ⓓgp /\
-                        s R_A0 = ⒹxTask /\
-                        s R_A3 = Ⓓa3 /\
+| 0x80000958 => Some (s V_MEM32 = base_mem /\ s R_GP = gp /\
+                        s R_A0 = xTask /\
+                        s R_A3 = a3 /\
                         cycle_count_of_trace t' = 0)
 | 0x800009e8 | 0x800009f0 => Some (time_of_eTaskGetState base_mem gp a3 xTask t)
 | _ => None end | _ => None end.
-
-Definition lifted_eTaskGetState : program :=
-    lift_riscv RTOSDemo_NoAsserts_Clz.
-
-(* We use simpl in a few convenient places: make sure it doesn't go haywire *)
-Arguments N.add _ _ : simpl nomatch.
-Arguments N.mul _ _ : simpl nomatch.
 
 Theorem eTaskGetState_timing:
   forall s t s' x' base_mem gp a3 xTask
          (ENTRY: startof t (x',s') = (Addr entry_addr, s))
          (MDL: models rvtypctx s)
-         (MEM: s V_MEM32 = Ⓜbase_mem)
-         (GP: s R_GP = Ⓓgp)
-         (A0: s R_A0 = ⒹxTask)
-         (A3: s R_A3 = Ⓓa3),
+         (MEM: s V_MEM32 = base_mem)
+         (GP: s R_GP = gp)
+         (A0: s R_A0 = xTask)
+         (A3: s R_A3 = a3),
   satisfies_all 
-    lifted_eTaskGetState
+    lifted_prog
     (eTaskGetState_timing_invs s base_mem gp a3 xTask)
     exits
   ((x',s')::t).
 Proof using.
     intros.
     apply prove_invs.
-    Local Ltac step := time rv_step.
+    Local Ltac step := time r5_step.
 
     simpl. rewrite ENTRY. unfold entry_addr. step. auto.
 
@@ -128,15 +121,9 @@ Proof using.
 
     destruct_inv 32 PRE.
     destruct PRE as (MEM & GP & A0 & A3 & Cycles).
-    repeat step.
-
-    { unfold time_of_eTaskGetState, pxCurrentTCB.
-        fold_big_subs. hammer. }
-
-    unfold time_of_eTaskGetState, pxCurrentTCB.
-        fold_big_subs. hammer.
-
-    par:
-        try solve [unfold time_of_eTaskGetState;
-        unfold pxCurrentTCB; fold_big_subs;
-        hammer].
+    do 4 step.
+      unfold pxCurrentTCB. hammer.
+      admit.
+    step. step. step. step. step. step.
+    (* The proof comes to a halt here (literally) due to step *)
+Abort.
