timing/examples/FreeRTOS/tasks/vTaskSwitchContext.v
@@ -29,7 +29,7 @@ Import Program_vTaskSwitchContext vTaskSwitchContextAuto.
    - Modifying shared memory
    - Performance optimization
 *)
-Definition uxSchedulerSuspended (gp : N) (mem : addr -> N) : N :=
+Definition uxSchedulerSuspended (gp : N) (mem : memory) : N :=
     mem Ⓓ[gp ⊖ 1952].
 
 (* The address of the doubleword in static memory that is nonzero when a task is
@@ -42,13 +42,13 @@ Definition addr_xYieldPendings (gp : N) : addr :=
 (* A pointer in static memory to the Current Task Control Block (TCB). The TCB
    is a data structure containing all essential information for managing a task.
 *)
-Definition pxCurrentTCB (gp : N) (mem : addr -> N) : N :=
+Definition pxCurrentTCB (gp : N) (mem : memory) : N :=
     mem Ⓓ[gp ⊖ 1896].
 
 (* The doubleword in static memory that records the highest priority out of all
    currently-ready tasks.
 *)
-Definition uxTopReadyPriority (gp : N) (mem : addr -> N) : N :=
+Definition uxTopReadyPriority (gp : N) (mem : memory) : N :=
     mem Ⓓ[gp ⊖ 1920].
 
 (* The address in static memory of a list of linked-lists that record all currently-
@@ -101,7 +101,7 @@ Definition smem_well_formed (gp : N) : Prop :=
    TCB or stack memory. Some of these assumptions can actually be proven due to 
    the boundaries of clz (count leading zeroes) being 0..32
 *)
-Definition pxCurrentTCB_noverlap_clz_static (gp : N) (mem : addr -> N) : Prop :=
+Definition pxCurrentTCB_noverlap_clz_static (gp : N) (mem : memory) : Prop :=
     ~ overlap 32
         (48 + pxCurrentTCB gp mem) 4
         (gp ⊖ 920 ⊕ (31 ⊖ clz (uxTopReadyPriority gp mem) 32) * 20) 4.
@@ -114,26 +114,26 @@ Definition clz_noverlap_smem (gp : N) mem : Prop :=
             (gp ⊖ 920 ⊕ (31 ⊖ clz (uxTopReadyPriority gp mem) 32) * 20) 4.
 
 (* The TCB doesn't overlap static memory or the stack frame *)
-Definition pxCurrentTCB_noverlap_static (gp : N) (mem : addr -> N) : Prop :=
+Definition pxCurrentTCB_noverlap_static (gp : N) (mem : memory) : Prop :=
     forall x len_x,
         static_buffer_lengths_in_bytes x = Some len_x ->
         ~ overlap 32
             (48 + pxCurrentTCB gp mem) 4
             (gp ⊖ x) len_x.
 
-Definition pxCurrentTCB_noverlap_stackframe (gp base_sp : N) (mem : addr -> N) : Prop :=
+Definition pxCurrentTCB_noverlap_stackframe (gp base_sp : N) (mem : memory) : Prop :=
     ~ overlap 32
         (48 + pxCurrentTCB gp mem) 4
         (base_sp ⊖ 16) 16.
 
 (* The address contained in the current TCB doesn't overlap with static memory
    or the stack frame *)
-Definition mem_pxCurrentTCB_noverlap_stackframe (gp base_sp : N) (mem : addr -> N) : Prop :=
+Definition mem_pxCurrentTCB_noverlap_stackframe (gp base_sp : N) (mem : memory) : Prop :=
     ~ overlap 32
         (mem Ⓓ[48 + pxCurrentTCB gp mem]) 4
         (base_sp ⊖ 16) 16.
 
-Definition mem_pxCurrentTCB_noverlap_static (gp : N) (mem : addr -> N) : Prop :=
+Definition mem_pxCurrentTCB_noverlap_static (gp : N) (mem : memory) : Prop :=
     forall x len_x,
         static_buffer_lengths_in_bytes x = Some len_x ->
         ~ overlap 32
@@ -142,25 +142,25 @@ Definition mem_pxCurrentTCB_noverlap_static (gp : N) (mem : addr -> N) : Prop :=
 
 (* Offsets into the address contained in the current TCB don't overlap with 
    the clz address or stack memory *)
-Definition offset_mem_pxCurrentTCB_noverlap_clz (gp : N) (mem : addr -> N) : Prop :=
+Definition offset_mem_pxCurrentTCB_noverlap_clz (gp : N) (mem : memory) : Prop :=
     forall k, k = 8 \/ k = 12 ->
         ~ overlap 32
             (k + mem Ⓓ[48 + pxCurrentTCB gp mem]) 4
             (gp ⊖ 920 ⊕ (31 ⊖ clz (uxTopReadyPriority gp mem) 32) * 20) 4.
 
-Definition clz_noverlap_sframe (gp base_sp : N) (mem : addr -> N) : Prop :=
+Definition clz_noverlap_sframe (gp base_sp : N) (mem : memory) : Prop :=
     ~ overlap 32 
         (base_sp ⊖ 16) 16
         (gp ⊖ 920 ⊕ (31 ⊖ clz (uxTopReadyPriority gp mem) 32) * 20) 4.
 
 (* An offset into the buffer at the clz address doesn't overlap with static
    memory or the stack frame *)
-Definition mem4_pxCurrentTCB_noverlap_stackframe (gp base_sp : N) (mem : addr -> N) : Prop :=
+Definition mem4_pxCurrentTCB_noverlap_stackframe (gp base_sp : N) (mem : memory) : Prop :=
         ~ overlap 32
         (base_sp ⊖ 16) 16
             (4 + mem Ⓓ[gp ⊖ 920 ⊕ (31 ⊖ clz (uxTopReadyPriority gp mem) 32) * 20]) 4.
 
-Definition mem4_pxCurrentTCB_noverlap_static (gp : N) (mem : addr -> N) : Prop :=
+Definition mem4_pxCurrentTCB_noverlap_static (gp : N) (mem : memory) : Prop :=
     forall x len_x,
         static_buffer_lengths_in_bytes x = Some len_x ->
         ~ overlap 32
@@ -169,12 +169,12 @@ Definition mem4_pxCurrentTCB_noverlap_static (gp : N) (mem : addr -> N) : Prop :
 
 (* An offset into the buffer at an offset into the buffer at the clz address 
    doesn't overlap with static memory or the stack frame *)
-Definition mem4_mem4_noverlap_stackframe (gp base_sp : N) (mem : addr -> N) :=
+Definition mem4_mem4_noverlap_stackframe (gp base_sp : N) (mem : memory) :=
     ~ overlap 32
         (base_sp ⊖ 16) 16
         (4 + mem Ⓓ[ 4 + mem Ⓓ[ gp ⊖ 920 ⊕ (31 ⊖ clz (uxTopReadyPriority gp mem) 32) * 20 ] ]) 4.
 
-Definition mem4_mem4_noverlap_static (gp : N) (mem : addr -> N) :=
+Definition mem4_mem4_noverlap_static (gp : N) (mem : memory) :=
     forall x len_x,
         static_buffer_lengths_in_bytes x = Some len_x ->
         ~ overlap 32
@@ -196,7 +196,7 @@ Definition common_noverlaps gp base_sp mem : Prop :=
     mem4_pxCurrentTCB_noverlap_stackframe gp base_sp mem /\
     mem4_pxCurrentTCB_noverlap_static gp mem.
 
-Definition time_of_vTaskSwitchContext (t : trace) (gp : N) (mem : addr -> N) : Prop :=
+Definition time_of_vTaskSwitchContext (t : trace) (gp : N) (mem : memory) : Prop :=
   cycle_count_of_trace t = (* total number of cycles equals... *)
     tlw +
     (* is the scheduler suspended *)
@@ -223,7 +223,7 @@ Definition time_of_vTaskSwitchContext (t : trace) (gp : N) (mem : addr -> N) : P
    The properties that we state help us prove the postcondition. We must prove
    each invariant throughout the proof. *)
 Definition vTaskSwitchContext_timing_invs (_ : store) (p : addr) 
-    (base_sp gp : N) (base_mem : addr -> N) (t:trace) : option Prop :=
+    (base_sp gp : N) (base_mem : memory) (t:trace) : option Prop :=
 match t with (Addr a, s) :: t' => match a with
     (* vApplicationStackOverflowHook *)
     (* NOTE : This function intentionally goes into an infinite loop when a
@@ -233,8 +233,8 @@ match t with (Addr a, s) :: t' => match a with
     | 0x8000e804 => Some True
     (* vTaskSwitchContext *)
     | 0x80001380 => Some (
-        exists mem, s V_MEM32 = Ⓜmem /\ s R_GP = Ⓓgp /\ s R_SP = Ⓓbase_sp 
-            /\ s R_A4 = Ⓓ(uxSchedulerSuspended gp base_mem) /\
+        exists mem, s V_MEM32 = mem /\ s R_GP = gp /\ s R_SP = base_sp 
+            /\ s R_A4 = (uxSchedulerSuspended gp base_mem) /\
             common_noverlaps gp base_sp mem /\
             mem4_mem4_noverlap_stackframe gp base_sp mem /\
             mem4_mem4_noverlap_static gp mem /\
@@ -248,8 +248,8 @@ match t with (Addr a, s) :: t' => match a with
             mem Ⓓ[ 4 + mem Ⓓ[ gp ⊖ 920 + (31 ⊖ clz (uxTopReadyPriority gp mem) 32) * 20 ] ] =
             base_mem Ⓓ[ 4 + base_mem Ⓓ[ gp ⊖ 920 + (31 ⊖ clz (uxTopReadyPriority gp base_mem) 32) * 20 ] ]  /\
         cycle_count_of_trace t' = tlw)
-    | 0x800013b4 => Some (exists mem, s V_MEM32 = Ⓜmem /\ 
-        s R_GP = Ⓓgp /\
+    | 0x800013b4 => Some (exists mem, s V_MEM32 = mem /\ 
+        s R_GP = gp /\
         common_noverlaps gp base_sp mem /\
         mem4_mem4_noverlap_stackframe gp base_sp mem /\
         mem4_mem4_noverlap_static gp mem /\
@@ -264,8 +264,8 @@ match t with (Addr a, s) :: t' => match a with
             base_mem Ⓓ[ 4 + base_mem Ⓓ[ gp ⊖ 920 + (31 ⊖ clz (uxTopReadyPriority gp base_mem) 32) * 20 ] ]  /\
         (uxSchedulerSuspended gp base_mem =? 0) = true /\
         cycle_count_of_trace t' = tlw + ttbeq + taddi + tsw + tsw + tlw + tlui + tsw + tlw + taddi + tlw)
-    | 0x800013bc => Some (exists mem, s V_MEM32 = Ⓜmem /\ 
-        s R_GP = Ⓓgp /\
+    | 0x800013bc => Some (exists mem, s V_MEM32 = mem /\ 
+        s R_GP = gp /\
         common_noverlaps gp base_sp mem /\
         mem4_mem4_noverlap_stackframe gp base_sp mem /\
         mem4_mem4_noverlap_static gp mem /\
@@ -280,8 +280,8 @@ match t with (Addr a, s) :: t' => match a with
             base_mem Ⓓ[ 4 + base_mem Ⓓ[ gp ⊖ 920 + (31 ⊖ clz (uxTopReadyPriority gp base_mem) 32) * 20 ] ]  /\
         (uxSchedulerSuspended gp base_mem =? 0) = true /\
         cycle_count_of_trace t' = tlw + ttbeq + taddi + tsw + tsw + tlw + tlui + tsw + tlw + taddi + tlw + tfbne + tlw)
-    | 0x800013c4 => Some (exists mem, s V_MEM32 = Ⓜmem /\ 
-        s R_GP = Ⓓgp /\
+    | 0x800013c4 => Some (exists mem, s V_MEM32 = mem /\ 
+        s R_GP = gp /\
         common_noverlaps gp base_sp mem /\
         mem4_mem4_noverlap_stackframe gp base_sp mem /\
         mem4_mem4_noverlap_static gp mem /\
@@ -297,8 +297,8 @@ match t with (Addr a, s) :: t' => match a with
         (uxSchedulerSuspended gp base_mem =? 0) = true /\
         cycle_count_of_trace t' = tlw + ttbeq + taddi + tsw + tsw + tlw + tlui + tsw + tlw + taddi + tlw + tfbne + tlw + tfbne + tlw
     )
-    | 0x800013cc => Some (exists mem, s V_MEM32 = Ⓜmem /\ 
-        s R_GP = Ⓓgp /\
+    | 0x800013cc => Some (exists mem, s V_MEM32 = mem /\ 
+        s R_GP = gp /\
         common_noverlaps gp base_sp mem /\
         mem4_mem4_noverlap_stackframe gp base_sp mem /\
         mem4_mem4_noverlap_static gp mem /\
@@ -314,11 +314,11 @@ match t with (Addr a, s) :: t' => match a with
         (uxSchedulerSuspended gp base_mem =? 0) = true /\
         cycle_count_of_trace t' = tlw + ttbeq + taddi + tsw + tsw + tlw + tlui + tsw + tlw + taddi + tlw + tfbne + tlw + tfbne + tlw + tfbne + tlw
     )
-    | 0x80001418 => Some (exists mem, s V_MEM32 = Ⓜmem /\ 
-        s R_GP = Ⓓgp /\
-        s R_A1 = Ⓓ(mem Ⓓ[4 + (gp ⊖ 924) ⊕ ((31 ⊖ (clz (uxTopReadyPriority gp mem) 32)) * 20)]) /\
-        s R_A2 = Ⓓ(addr_pxReadyTasksLists gp ⊕ ((31 ⊖ (clz (uxTopReadyPriority gp mem) 32)) * 20)) /\
-        s R_A5 = Ⓓ((gp ⊖ 916) ⊕ (31 ⊖ clz (uxTopReadyPriority gp mem) 32) * 20) /\
+    | 0x80001418 => Some (exists mem, s V_MEM32 = mem /\ 
+        s R_GP = gp /\
+        s R_A1 = (mem Ⓓ[4 + (gp ⊖ 924) ⊕ ((31 ⊖ (clz (uxTopReadyPriority gp mem) 32)) * 20)]) /\
+        s R_A2 = (addr_pxReadyTasksLists gp ⊕ ((31 ⊖ (clz (uxTopReadyPriority gp mem) 32)) * 20)) /\
+        s R_A5 = ((gp ⊖ 916) ⊕ (31 ⊖ clz (uxTopReadyPriority gp mem) 32) * 20) /\
         common_noverlaps gp base_sp mem /\
         uxTopReadyPriority gp mem = uxTopReadyPriority gp base_mem /\
         mem Ⓓ[ gp ⊖ 920 + (31 ⊖ clz (uxTopReadyPriority gp mem) 32) * 20 ] =
@@ -332,17 +332,13 @@ match t with (Addr a, s) :: t' => match a with
 | _ => None
 end.
 
-Goal forall gp mem, tlw + ttbeq + taddi + tsw + tsw + tlw + tlui + tsw + tlw + taddi + tlw + tfbne + tlw +
-tfbne + tlw + tfbne + tlw + ttbeq + tlw + taddi + tclz (uxTopReadyPriority gp mem) = 0.
-    intros. psimpl.
-
 Theorem vTaskSwitchContext_timing:
   forall s p t s' x' gp sp mem
          (ENTRY: startof t (x',s') = (Addr entry_addr,s))
          (MDL: models rvtypctx s)
-         (GP : s R_GP = Ⓓgp)
-         (SP : s R_SP = Ⓓsp)
-         (MEM : s V_MEM32 = Ⓜmem)
+         (GP : s R_GP = gp)
+         (SP : s R_SP = sp)
+         (MEM : s V_MEM32 = mem)
          (NOVERLAPS : common_noverlaps gp sp mem)
          (MEM4_NOVERLAPS : 
             mem4_mem4_noverlap_stackframe gp sp mem /\
@@ -363,7 +359,7 @@ Proof using.
     (* Set up our proof environment *)
     intros.
     apply prove_invs.
-    Local Ltac step := time rv_step.
+    Local Ltac step := tstep r5_step.
 
     Local Ltac unfold_vTaskSwitchContext :=
         unfold uxSchedulerSuspended, __global_size,
@@ -419,12 +415,12 @@ Proof using.
             repeat rewrite <- getmem_mod_l with (a := _ + _).
             rewrite getmem_mod_l.
             replace (clz _ 32) with (clz (uxTopReadyPriority gp mem) 32) by memsolve mem gp sp.
-            replace ((mem [Ⓓgp ⊖ 1932 := 0 ] [Ⓓsp ⊖ 8 := n ] [Ⓓsp ⊖ 4 := n0 ])
+            replace ((mem [Ⓓgp ⊖ 1932 := 0 ] [Ⓓsp ⊖ 8 := s' R_S0 ] [Ⓓsp ⊖ 4 := s' R_RA ])
                 Ⓓ[ gp ⊖ 920 ⊕ (31 ⊖ clz (uxTopReadyPriority gp mem) 32) * 20 ]) with
                 (mem Ⓓ[ gp ⊖ 920 ⊕ (31 ⊖ clz (uxTopReadyPriority gp mem) 32) * 20 ]); cycle 1.
                 memsolve mem gp sp.
             rewrite getmem_mod_l.
-            replace ((mem [Ⓓgp ⊖ 1932 := 0 ] [Ⓓsp ⊖ 8 := n ] [Ⓓsp ⊖ 4 := n0 ])
+            replace ((mem [Ⓓgp ⊖ 1932 := 0 ] [Ⓓsp ⊖ 8 := s' R_S0 ] [Ⓓsp ⊖ 4 := s' R_RA ])
                 Ⓓ[ 4 + mem Ⓓ[ gp ⊖ 920 ⊕ (31 ⊖ clz (uxTopReadyPriority gp mem) 32) * 20 ] ]) with
                 (mem Ⓓ[ 4 + mem Ⓓ[ gp ⊖ 920 ⊕ (31 ⊖ clz (uxTopReadyPriority gp mem) 32) * 20 ] ]); cycle 1.
                 memsolve mem gp sp. now eapply MEM4_PCT_NOL_STATIC.
@@ -436,8 +432,7 @@ Proof using.
                 [psimpl; lia|auto].
         }
         hammer.
-    unfold time_of_vTaskSwitchContext.
-        hammer.
+    hammer.
 
     (* 0x800013c8 *)
     destruct PRE as (mem & MEM & GP & NOVERLAPS & MEM4_MEM4_NOL_SFRAME
@@ -476,6 +471,7 @@ Proof using.
     repeat step.
         eexists. split. reflexivity.
         repeat split; auto.
+        (* TODO : memsolve broken ? *)
         1-15: try solve [noverlap_prepare gp sp; memsolve mem gp sp].
         {
             noverlap_prepare gp sp.
