timing/examples/FreeRTOS/tasks/prvResetNextTaskUnblockTime.v
@@ -20,7 +20,7 @@ Module RISCVTiming := RISCVTiming cpu Program_prvResetNextTaskUnblockTime.
 Module prvResetNextTaskUnblockTimeAuto := RISCVTimingAutomation RISCVTiming.
 Import Program_prvResetNextTaskUnblockTime prvResetNextTaskUnblockTimeAuto.
 
-Definition time_of_prvResetNextTaskUnblockTime (mem : addr -> N) (gp : N) (t : trace) :=
+Definition time_of_prvResetNextTaskUnblockTime (mem : memory) (gp : N) (t : trace) :=
     cycle_count_of_trace t =
         tlw + tlw +
         (if mem Ⓓ[mem Ⓓ[gp ⊖ 1900]] =? 0 then 
@@ -29,10 +29,10 @@ Definition time_of_prvResetNextTaskUnblockTime (mem : addr -> N) (gp : N) (t : t
             ttbne + tlw + tlw + tlw + tjal) +
         tsw + tjalr.
 
-Definition prvResetNextTaskUnblockTime_timing_invs (s : store) (base_mem : addr -> N) (gp : N)
+Definition prvResetNextTaskUnblockTime_timing_invs (s : store) (base_mem : memory) (gp : N)
     (t:trace) : option Prop :=
 match t with (Addr a, s) :: t' => match a with
-| 0x80000478 => Some (s V_MEM32 = Ⓜbase_mem /\ s R_GP = Ⓓgp /\ cycle_count_of_trace t' = 0)
+| 0x80000478 => Some (s V_MEM32 = base_mem /\ s R_GP = gp /\ cycle_count_of_trace t' = 0)
 | 0x8000048c => Some (time_of_prvResetNextTaskUnblockTime base_mem gp t)
 | _ => None end | _ => None end.
 
@@ -40,8 +40,8 @@ Theorem prvResetNextTaskUnblockTime_timing:
   forall s t s' x' base_mem gp
          (ENTRY: startof t (x',s') = (Addr entry_addr, s))
          (MDL: models rvtypctx s)
-         (MEM: s V_MEM32 = Ⓜbase_mem)
-         (GP: s R_GP = Ⓓgp),
+         (MEM: s V_MEM32 = base_mem)
+         (GP: s R_GP = gp),
   satisfies_all 
     lifted_prog
     (prvResetNextTaskUnblockTime_timing_invs s base_mem gp)
@@ -50,7 +50,7 @@ Theorem prvResetNextTaskUnblockTime_timing:
 Proof using.
     intros.
     apply prove_invs.
-    Local Ltac step := time rv_step.
+    Local Ltac step := tstep r5_step.
 
     simpl. rewrite ENTRY. unfold entry_addr. step. auto.
 
@@ -63,11 +63,7 @@ Proof using.
     destruct_inv 32 PRE.
 
     destruct PRE as (MEM & GP & Cycles).
-    repeat step; fold_big_subs.
-    unfold time_of_prvResetNextTaskUnblockTime.
-        hammer.
-    unfold time_of_prvResetNextTaskUnblockTime.
-        hammer.
+    repeat step; fold_big_subs; hammer.
 Qed.
 
 End TimingProof.
