timing/examples/data_structures/array/bubble_sort/loose_bound/bubble_sort_theta_n2_proof.v
@@ -31,7 +31,7 @@ Module RISCVTiming := RISCVTiming cpu Program_bubble_sort_theta_n2.
 Module bubble_sort_theta_n2Auto := RISCVTimingAutomation RISCVTiming.
 Import Program_bubble_sort_theta_n2 bubble_sort_theta_n2Auto.
 
-Definition time_of_bubble_sort_theta_n2 (mem : addr -> N) 
+Definition time_of_bubble_sort_theta_n2 (mem : memory) 
         (arr : addr) (len : N) (t : trace) :=
     (* ----------------------------------------- *)
     (* lower bound, return if len = 0 *)
@@ -60,19 +60,19 @@ Definition time_of_bubble_sort_theta_n2 (mem : addr -> N)
     (* return *)
     tjalr.
 
-Definition bubble_sort_theta_n2_timing_invs (s : store) (base_mem : addr -> N)
+Definition bubble_sort_theta_n2_timing_invs (s : store) (base_mem : memory)
     (arr : addr) (len : N) (_a5 : N) (t:trace) : option Prop :=
 match t with (Addr a, s) :: t' => match a with
-| 0x1e4 => Some (s V_MEM32 = Ⓜbase_mem /\ 
-                    s R_A0 = Ⓓarr /\ s R_A1 = Ⓓlen /\
-                    s R_A5 = Ⓓ_a5 /\
+| 0x1e4 => Some (s V_MEM32 = base_mem /\ 
+                    s R_A0 = arr /\ s R_A1 = len /\
+                    s R_A5 = _a5 /\
                     arr + 4 * len < 2^32 /\
                     cycle_count_of_trace t' = 0)
-| 0x1f0 => Some (exists mem a4, s V_MEM32 = Ⓜmem /\
-                   s R_A0 = Ⓓarr /\ s R_A1 = Ⓓlen /\
-                   s R_A3 = Ⓓ(arr + 4 * len) /\
+| 0x1f0 => Some (exists mem a4, s V_MEM32 = mem /\
+                   s R_A0 = arr /\ s R_A1 = len /\
+                   s R_A3 = (arr + 4 * len) /\
                    (* a4 is outer loop counter *)
-                   s R_A4 = Ⓓa4 /\
+                   s R_A4 = a4 /\
                    a4 <= len /\
                    arr + 4 * len < 2^32 /\
                    tslli 2 + tadd + taddi <=
@@ -93,12 +93,12 @@ match t with (Addr a, s) :: t' => match a with
                        taddi + tjal
                    )
             )
-| 0x214 => Some (exists mem a4 inner_loop_count, s V_MEM32 = Ⓜmem /\
-                   s R_A0 = Ⓓarr /\ s R_A1 = Ⓓlen /\
-                   s R_A3 = Ⓓ(arr + 4 * len) /\
+| 0x214 => Some (exists mem a4 inner_loop_count, s V_MEM32 = mem /\
+                   s R_A0 = arr /\ s R_A1 = len /\
+                   s R_A3 = (arr + 4 * len) /\
                    (* a4 is outer loop counter *)
-                   s R_A4 = Ⓓa4 /\
-                   s R_A5 = Ⓓ(arr + 4 * (1 + inner_loop_count)) /\
+                   s R_A4 = a4 /\
+                   s R_A5 = (arr + 4 * (1 + inner_loop_count)) /\
                    1 + inner_loop_count <= len /\
                    (* this is here to handle the inductive case where 
                       inner_loop_count is incremented *)
@@ -140,10 +140,10 @@ Theorem bubble_sort_theta_n2_timing:
          (ENTRY: startof t (x',s') = (Addr entry_addr, s))
          (MDL: models rvtypctx s)
          (* bindings *)
-         (MEM: s V_MEM32 = Ⓜbase_mem)
-         (A0: s R_A0 = Ⓓarr)
-         (A2: s R_A1 = Ⓓlen)
-         (A5: s R_A5 = Ⓓa5)
+         (MEM: s V_MEM32 = base_mem)
+         (A0: s R_A0 = arr)
+         (A2: s R_A1 = len)
+         (A5: s R_A5 = a5)
          (* array must fit inside the address space without wrapping *)
          (* this shouldn't be necessary but makes the proof easy *)
          (ARR_VALID: arr + 4 * len < 2^32),
@@ -155,7 +155,7 @@ Theorem bubble_sort_theta_n2_timing:
 Proof using.
     intros.
     apply prove_invs.
-    Local Ltac step := time rv_step.
+    Local Ltac step := tstep r5_step.
 
     simpl. rewrite ENTRY. unfold entry_addr. step.
     now repeat split.
